Veritas.MultiSet.fsti
@@ -95,3 +95,6 @@ val lemma_add_size (#a:eqtype) (s:mset a) (x:a):
   Lemma (requires True)
         (ensures (size (add_elem s x) = size s + 1))
         [SMTPat (add_elem s x)]
+
+val lemma_add_elem (#a:eqtype) (s: seq a) (x: a):
+  Lemma (seq2mset (append1 s x) == add_elem (seq2mset s) x)
